FE310 MMIO: allow SPI1

src/riscv/Platform/FE310ExtSpec.v
@@ -14,9 +14,10 @@ Section MMIO.
   Definition isPRCI (addr: word): Prop := Ox"10008000" <= word.unsigned addr < Ox"10010000".
   Definition isGPIO0(addr: word): Prop := Ox"10012000" <= word.unsigned addr < Ox"10013000".
   Definition isUART0(addr: word): Prop := Ox"10013000" <= word.unsigned addr < Ox"10014000".
+  Definition isSPI1 (addr: word): Prop := Ox"10024000" <= word.unsigned addr < Ox"10025000".
 
   Instance FE310_mmio: MMIOSpec := {|
-    isMMIOAddr(addr: word) := isOTP addr \/ isPRCI addr \/ isGPIO0 addr \/ isUART0 addr;
+    isMMIOAddr(addr: word) := isOTP addr \/ isPRCI addr \/ isGPIO0 addr \/ isUART0 addr \/ isSPI1 addr;
     isMMIOAligned(n: nat)(addr: word) := n = 4%nat /\ (word.unsigned addr) mod 4 = 0;
   |}.
 
